src/proof/well_formed.v
@@ -9,44 +9,63 @@ From proof Require Export deepcopy.
 Section proof.
 Context `{hG: !heapGS Σ} {go_ctx: GoContext}.
 
+Definition has_controller_parent (oslice: slice.t) (os: list v1.OwnerReference.t) (o: v1.OwnerReference.t) (c: bool) : iProp Σ :=
+  oslice ↦*□ os ∗ ⌜ o ∈ os ⌝ ∗ o.(v1.OwnerReference.Controller') ↦□ c ∗ ⌜ c = true ⌝.
+
+Definition has_controller_parent_of (oslice: slice.t) (uid: go_string) : iProp Σ :=
+  ∃ os o c, has_controller_parent oslice os o c ∗ ⌜ o.(v1.OwnerReference.UID') = uid ⌝.
+
 Definition object_meta_well_formed (m: v1.ObjectMeta.t) : iProp Σ :=
-  "uid_well_formed" ∷ ⌜ m.(v1.ObjectMeta.UID') ≠ "_ORPHAN_POD"%go ⌝.
+  "%uid_well_formed" ∷ ⌜ m.(v1.ObjectMeta.UID') ≠ "_ORPHAN_POD"%go ⌝ ∗
+  (* Kubernetes guarantees there is only one element in OwnerReferences' whose Controller' is true,
+  but here we only need a weaker specification saying that if there are two controller parents then they are the same. *)
+  "#at_most_one_controller_parent" ∷ □ ∀ uid1 uid2,
+    has_controller_parent_of m.(v1.ObjectMeta.OwnerReferences') uid1 -∗ 
+      has_controller_parent_of m.(v1.ObjectMeta.OwnerReferences') uid2 -∗
+        ⌜ uid1 = uid2 ⌝.
 
 Axiom pod_spec_well_formed: v1.PodSpec.t → iProp Σ.
+Global Instance pod_spec_well_formed_persistent spec : Persistent (pod_spec_well_formed spec).
+Proof. Admitted.
 
 Axiom pod_status_well_formed: v1.PodStatus.t → iProp Σ.
+Global Instance pod_status_well_formed_persistent status : Persistent (pod_status_well_formed status).
+Proof. Admitted.
 
 Definition pod_well_formed (pod: v1.Pod.t) : iProp Σ :=
-  "pod_metadata_well_formed" ∷ object_meta_well_formed pod.(v1.Pod.ObjectMeta') ∗
-  "pod_spec_well_formed" ∷ pod_spec_well_formed pod.(v1.Pod.Spec') ∗
-  "pod_status_well_formed" ∷ pod_status_well_formed pod.(v1.Pod.Status').
+  "#pod_metadata_well_formed" ∷ object_meta_well_formed pod.(v1.Pod.ObjectMeta') ∗
+  "#pod_spec_well_formed" ∷ pod_spec_well_formed pod.(v1.Pod.Spec') ∗
+  "#pod_status_well_formed" ∷ pod_status_well_formed pod.(v1.Pod.Status').
 
 Definition pod_nn_well_formed (pod: v1.Pod.t) (namespace name: go_string) : iProp Σ :=
   "%namespace_match" ∷ ⌜ pod.(v1.Pod.ObjectMeta').(v1.ObjectMeta.Namespace') = namespace ⌝ ∗
   "%name_match" ∷ ⌜ pod.(v1.Pod.ObjectMeta').(v1.ObjectMeta.Name') = name ⌝ ∗
-  "pod_well_formed" ∷ pod_well_formed pod.
+  "#pod_well_formed" ∷ pod_well_formed pod.
 
 Definition object_meta_to_create_well_formed (m: v1.ObjectMeta.t) : iProp Σ :=
-  "generatename_not_empty_if_name_empty" ∷ ⌜ m.(v1.ObjectMeta.Name') = ""%go → m.(v1.ObjectMeta.GenerateName') ≠ ""%go ⌝.
+  "%generatename_not_empty_if_name_empty" ∷ ⌜ m.(v1.ObjectMeta.Name') = ""%go → m.(v1.ObjectMeta.GenerateName') ≠ ""%go ⌝.
 
 Axiom pod_spec_to_create_well_formed: v1.PodSpec.t → iProp Σ.
+Global Instance pod_spec_to_create_well_formed_persistent spec : Persistent (pod_spec_to_create_well_formed spec).
+Proof. Admitted.
 
 Axiom pod_status_to_create_well_formed: v1.PodStatus.t → iProp Σ.
+Global Instance pod_status_to_create_well_formed_persistent status : Persistent (pod_status_to_create_well_formed status).
+Proof. Admitted.
 
 Definition pod_to_create_well_formed (pod: v1.Pod.t) : iProp Σ :=
-  "pod_metadata_to_create_well_formed" ∷ object_meta_to_create_well_formed pod.(v1.Pod.ObjectMeta') ∗
-  "pod_spec_to_create_well_formed" ∷ pod_spec_to_create_well_formed pod.(v1.Pod.Spec') ∗
-  "pod_status_to_create_well_formed" ∷ pod_status_to_create_well_formed pod.(v1.Pod.Status').
+  "#pod_metadata_to_create_well_formed" ∷ object_meta_to_create_well_formed pod.(v1.Pod.ObjectMeta') ∗
+  "#pod_spec_to_create_well_formed" ∷ pod_spec_to_create_well_formed pod.(v1.Pod.Spec') ∗
+  "#pod_status_to_create_well_formed" ∷ pod_status_to_create_well_formed pod.(v1.Pod.Status').
 
 Definition pod_to_create_nn_well_formed (pod: v1.Pod.t) (namespace name: go_string) : iProp Σ :=
   "%namespace_match" ∷ ⌜ pod.(v1.Pod.ObjectMeta').(v1.ObjectMeta.Namespace') = namespace ⌝ ∗
   "%name_match" ∷ ⌜ pod.(v1.Pod.ObjectMeta').(v1.ObjectMeta.Name') = name ⌝ ∗
-  "pod_to_create_well_formed" ∷ pod_to_create_well_formed pod.
-
+  "#pod_to_create_well_formed" ∷ pod_to_create_well_formed pod.
 
 Definition replicaset_well_formed (rs: v1.ReplicaSet.t) : iProp Σ :=
   object_meta_well_formed rs.(v1.ReplicaSet.ObjectMeta') ∗
-  ∃ (v: w32), rs.(v1.ReplicaSet.Spec').(v1.ReplicaSetSpec.Replicas') ↦ v ∗ ⌜ 0 ≤ sint.Z v ⌝.
+  ∃ (v: w32), rs.(v1.ReplicaSet.Spec').(v1.ReplicaSetSpec.Replicas') ↦□ v ∗ ⌜ 0 ≤ sint.Z v ⌝.
 
 Definition replicaset_nn_well_formed (rs: v1.ReplicaSet.t) (namespace name: go_string) : iProp Σ :=
   ⌜ rs.(v1.ReplicaSet.ObjectMeta').(v1.ObjectMeta.Namespace') = namespace ⌝ ∗
